[minor] 'Beautified' the formatting

src/Kind.v
@@ -1,5 +1,5 @@
-Require Export Expression.
-
+Require Import Expression.
+Require Import Util.
 (**
 Definition. The set [K] of lambda-kinds is defined
 inductively as follows:
@@ -10,7 +10,25 @@ inductively as follows:
   then [KLam x:A.B] is in [K].
 *)
 Inductive kind : Type :=
- | kappa : kind                           (* kind constant *)
- | KLam : Expression.exp -> kind -> kind. (* lambda kind *)
+ | kappa : kind                (* kind constant *)
+ | KLam : exp -> kind -> kind. (* lambda kind *)
 
+(**
+Theorem. If [k] is a Lambda-Kind, then either
+[k = kappa] or [k = KLam t k'] where [t] is some [exp]
+and [k'] is another Lambda-Kind.
 
+(As a consequence, it makes sense to talk about the
+"length" of a [kind] by counting the number of [KLam]
+constants that appear.)
+*)
+Theorem canonical_form_of_kinds :
+ forall k : kind, k = kappa \/ (exists (t : exp) (k' : kind), k = KLam t k').
+Proof.
+  intuition.
+  induction k.
+  (* Case: k = kappa *)
+  - left. reflexivity.
+  (* Case: k = KLam e k *)
+  - right. eauto .
+Qed.
