src/Lexer.v
@@ -1,14 +1,15 @@
 (**
 This just transforms "pretty print" notation to internal
-de Bruijn indices.
+de Bruijn indices. It's probably the most involved code
+that has the least to do with the actual type theoretic
+machinery.
 *)
 Require Import String.
 Require Export Coq.Lists.List.
 Require Export Coq.Arith.Compare_dec.
 Require Export Coq.Arith.EqNat.
 Require Export Util.
-Require Import ltlc.
-Import Expression.
+Require Import Expression.
 
 (** 
 For denaming some pretty-printed lambda expression into our
@@ -22,7 +23,7 @@ Inductive pterm : Type :=
  | App : pterm -> pterm -> pterm.
 
 (** The free variables in a given [pterm]. *)
-Fixpoint FV (t:pterm) : list string :=
+Fixpoint FV (t:pterm): list string :=
   match t with
   | tau => nil
   | Var s => s::nil
@@ -30,6 +31,10 @@ Fixpoint FV (t:pterm) : list string :=
   | App t1 t2 => append (FV t1) (FV t2)
   end.
 
+(** A [context] for pretty print reasons is a list of
+declarations, which themselves are ordered pairs of a 
+[string] identifier, and its corresponding [pterm] "type".
+*)
 Definition context := list (string * pterm).
 End PrettyTerm.
 
@@ -39,85 +44,89 @@ Notation "` x" := (if string_dec x "tau"
 Notation "\ x t ~> M" := (PrettyTerm.Lam x t M) (at level 30).
 Infix "$" := PrettyTerm.App (at level 25, left associativity).
 
-Example FV_ex1:
-  PrettyTerm.FV (`"f" $ `"g" $ `"h" $ `"i")
-  = "f"%string :: "g"%string :: "h"%string :: "i"%string :: nil.
+(* Unit tests for [FV] *)
+Example FV_ex1 :
+  PrettyTerm.FV (`"f" $ `"g" $ `"h" $ `"i") =
+  "f"%string :: "g"%string :: "h"%string :: "i"%string :: nil.
 Proof. reflexivity. Qed.
 
 Example prettier_left_assoc_ex1 :
- `"f" $ `"g" $ `"h" $ `"i"
-= (PrettyTerm.App
-    (PrettyTerm.App 
-      (PrettyTerm.App
-        (PrettyTerm.Var "f")
-        (PrettyTerm.Var "g"))
-      (PrettyTerm.Var "h"))
-    (PrettyTerm.Var "i")).
+  `"f" $ `"g" $ `"h" $ `"i" =
+  PrettyTerm.App
+    (PrettyTerm.App
+       (PrettyTerm.App (PrettyTerm.Var "f") (PrettyTerm.Var "g"))
+       (PrettyTerm.Var "h")) (PrettyTerm.Var "i").
 Proof.
   simpl. reflexivity.
 Qed.
 
 Example prettier_ex2 :
-  (\"f" `"tau" ~> `"f" $ \"x" `"tau" ~> `"x" $ `"y") =
-  PrettyTerm.Lam "f"
-    PrettyTerm.tau
-    (PrettyTerm.App
-      (PrettyTerm.Var "f")
-      (PrettyTerm.Lam "x" PrettyTerm.tau
-        (PrettyTerm.App
-          (PrettyTerm.Var "x")
-          (PrettyTerm.Var "y")))).
+  \ "f" `"tau" ~> `"f" $ (\ "x" `"tau" ~> `"x" $ `"y") =
+  PrettyTerm.Lam "f" PrettyTerm.tau
+    (PrettyTerm.App (PrettyTerm.Var "f")
+       (PrettyTerm.Lam "x" PrettyTerm.tau
+          (PrettyTerm.App (PrettyTerm.Var "x") (PrettyTerm.Var "y")))).
 Proof. simpl. reflexivity. Qed.
 
-Fixpoint lookup (s: string) (ls: list (string * nat)) : option nat :=
+Fixpoint lookup (s : string) (ls : list (string * nat)): 
+option nat :=
   match ls with
   | nil => None
   | (x, n) :: t => if string_dec x s then Some n else lookup s t
   end.
 
 (** Pushes the depth one layer, introduces a "new" variable [s]. *)
-Fixpoint hide (s: string) (ls: list (string * nat)) : list (string * nat) :=
+Fixpoint hide (s : string) (ls : list (string * nat)): 
+list (string * nat) :=
   match ls with
   | nil => (s, 0) :: nil
-  | (x, n) :: t => if string_dec x s
-                   then (x, 0) :: hide s t
-                   else (x, n + 1) :: hide s t
+  | (x, n) :: t =>
+      if string_dec x s then (x, 0) :: hide s t else (x, n + 1) :: hide s t
   end.
 
-Fixpoint dename' (t: PrettyTerm.pterm) (binds: list (string * nat)) : exp :=
+Fixpoint dename' (t : PrettyTerm.pterm) (binds : list (string * nat)): exp :=
   match t with
   | PrettyTerm.tau => tau
-  | PrettyTerm.Var s => match lookup s binds with
-             | Some n => EVar n
-             | None => EVar 0
-             end
-  | PrettyTerm.Lam s t b => ELam (dename' t (hide s binds)) (dename' b (hide s binds))
-  | PrettyTerm.App t1 t2 => EApp (dename' t1 binds) (dename' t2 binds) 
-end.
+  | PrettyTerm.Var s =>
+      match lookup s binds with
+      | Some n => EVar n
+      | None => EVar 0
+      end
+  | PrettyTerm.Lam s t b =>
+      ELam (dename' t (hide s binds)) (dename' b (hide s binds))
+  | PrettyTerm.App t1 t2 => EApp (dename' t1 binds) (dename' t2 binds)
+  end.
 
 (** Given a list [identifiers] of free variables, and a list [binds] of
     binds to de Bruijn indices, update it adding values for the free variables. *)
-Fixpoint FV_binds (identifiers: list string) (binds: list (string * nat)) : list (string * nat) :=
+Fixpoint FV_binds (identifiers : list string) (binds : list (string * nat)):
+list (string * nat) :=
   match identifiers with
   | nil => binds
-  | x::tl => match lookup x binds with
-             | Some n => FV_binds tl binds
-             | None => FV_binds tl (cons (x, length binds) binds)
-             end
+  | x :: tl =>
+      match lookup x binds with
+      | Some n => FV_binds tl binds
+      | None => FV_binds tl (cons (x, length binds) binds)
+      end
   end.
 
-Fixpoint context_binds' (Gamma: PrettyTerm.context) (binds: list (string * nat)) : list (string * nat) :=
+Fixpoint context_binds' (Gamma : PrettyTerm.context)
+(binds : list (string * nat)): list (string * nat) :=
   match Gamma with
   | nil => binds
-  | (x, _)::tl => match lookup x binds with
-                  | Some n => context_binds' tl binds
-                  | None => context_binds' tl (cons (x, length binds) binds)
-                  end
+  | (x, _) :: tl =>
+      match lookup x binds with
+      | Some n => context_binds' tl binds
+      | None => context_binds' tl (cons (x, length binds) binds)
+      end
   end.
 
-Definition context_binds (Gamma: PrettyTerm.context) : list (string * nat) :=
-  context_binds' (rev Gamma) nil.
+(** Given a [context Gamma = (xN,type_N), ..., (x1, type_1)] produce a lookup
+    map for the variables and identifiers to convert to de Bruijn indices. *)
+Definition context_binds (Gamma : PrettyTerm.context) :
+  list (string * nat) := context_binds' (rev Gamma) nil.
 
+(* Unit tests for the [context_binds] *)
 Open Scope string_scope.
 Example context_binds_ex1 :
   context_binds (cons ("f", PrettyTerm.tau) nil) = ("f", 0) :: nil.
@@ -126,64 +135,71 @@ Proof.
 Qed.
 
 Example context_binds_ex2 :
-  context_binds (cons ("f", PrettyTerm.tau) (cons ("g", PrettyTerm.tau) (cons ("f", PrettyTerm.tau) nil)))
-  = ("g", 1) :: ("f", 0) :: nil.
+  context_binds
+    (cons ("f", PrettyTerm.tau)
+       (cons ("g", PrettyTerm.tau) (cons ("f", PrettyTerm.tau) nil))) =
+  ("g", 1) :: ("f", 0) :: nil.
 Proof.
   reflexivity.
 Qed.
 
 Example fv_binds_context_binds_ex1 :
   FV_binds (PrettyTerm.FV (`"f" $ `"g" $ `"f"))
-           (context_binds (cons ("g", PrettyTerm.tau) nil))
-  = ("f", 1) :: ("g", 0) :: nil.
+    (context_binds (cons ("g", PrettyTerm.tau) nil)) =
+  ("f", 1) :: ("g", 0) :: nil.
 Proof.
   reflexivity.
 Qed.
 Close Scope string_scope.
 
+(** Given a [PrettyTerm.pterm] without a [context], convert it
+    into a [exp] using de Bruijn indices. *)
 Definition dename (t : PrettyTerm.pterm) : exp :=
-dename' t (FV_binds (PrettyTerm.FV t) nil).
+  dename' t (FV_binds (PrettyTerm.FV t) nil).
 
-Fixpoint deconstruct_context (c: PrettyTerm.context)
-                             (binds : list (string * nat))
-                             : list exp
-:= match c with
-   | nil => nil
-   | (x, t)::ctxt => cons (dename' t binds) (deconstruct_context ctxt binds)
-   end.
+(** If we have a given [context Gamma], then we want to convert it into
+    a [list exp] which binds to de Bruijn indices. *)
+Fixpoint deconstruct_context (c : PrettyTerm.context)
+(binds : list (string * nat)): list exp :=
+  match c with
+  | nil => nil
+  | (x, t) :: ctxt => cons (dename' t binds) (deconstruct_context ctxt binds)
+  end.
 
 (** Claim: Let [c = f : tau, h : \g:tau~>f], then
     [deconstruct_context c (context_binds c) = Elam tau f :: tau].
 *)
 Example deconstruct_context_ex1 :
-  let c := (snoc ("f"%string, `"tau") 
-                 (cons ("h"%string, \"g" `"tau" ~> `"f") nil))
-  in deconstruct_context c (context_binds c)
-  = (ELam tau (EVar 1)) :: tau :: nil.
+  let c :=
+    snoc ("f"%string, `"tau") (cons ("h"%string, \ "g" `"tau" ~> `"f") nil) in
+  deconstruct_context c (context_binds c) = ELam tau (EVar 1) :: tau :: nil.
 Proof. reflexivity. Qed.
 
 (** Claim: Let [c = h : \g:tau~>f, g : tau, f : tau], then
     [deconstruct_context c (context_binds c) = Elam tau f :: tau :: tau].
 *)
 Example deconstruct_context_ex2 :
-  let c := (snoc ("f"%string, `"tau") 
-                 (snoc ("g"%string, `"tau")
-                       (cons ("h"%string, \"x" `"g" ~> `"f") nil)))
-  in deconstruct_context c (context_binds c)
-  = ELam (EVar 2) (EVar 1) :: tau :: tau :: nil.
+  let c :=
+    snoc ("f"%string, `"tau")
+      (snoc ("g"%string, `"tau") (cons ("h"%string, \ "x" `"g" ~> `"f") nil)) in
+  deconstruct_context c (context_binds c) =
+  ELam (EVar 2) (EVar 1) :: tau :: tau :: nil.
 Proof. reflexivity. Qed.
 
-Definition dename_with_context (c: PrettyTerm.context)
-                               (t: PrettyTerm.pterm)
-                               : context * exp
-:= let binds := (FV_binds (PrettyTerm.FV t) (context_binds c))
-   in (deconstruct_context c binds, dename' t binds).
+(** Convert a [PrettyTerm.pterm] in a given [PrettyTerm.context] to
+    a pair [context, exp] using de Bruijn indices. Free Variables are
+    handled properly.
+*)
+Definition dename_with_context (c : PrettyTerm.context)
+  (t : PrettyTerm.pterm) : context * exp :=
+  let binds := FV_binds (PrettyTerm.FV t) (context_binds c) in
+  (deconstruct_context c binds, dename' t binds).
 
+(* Unit tests for [dename_with_context] *)
 Open Scope string_scope.
 Example dename_with_context_ex1 :
-  dename_with_context (cons ("g", PrettyTerm.tau) nil)
-                      (`"f" $ `"g" $ `"f")
-  = (tau :: nil, EApp (EApp (EVar 1) (EVar 0)) (EVar 1)).
+  dename_with_context (cons ("g", PrettyTerm.tau) nil) (`"f" $ `"g" $ `"f") =
+  (tau :: nil, EApp (EApp (EVar 1) (EVar 0)) (EVar 1)).
 Proof.
   reflexivity.
 Qed.
