src/Util.v
@@ -4,47 +4,118 @@ Require Export Coq.Arith.Compare_dec.
 Require Export Coq.Arith.EqNat.
 
 (* Add a single element to the end of the list *)
-Fixpoint snoc {A: Type} (x: A) (xx: list A) : list A :=
- match xx with 
- | nil       => x :: nil
- | y :: xs'  => y :: snoc x xs'
- end.
+Fixpoint snoc {A : Type} (x : A) (xx : list A): list A :=
+  match xx with
+  | nil => x :: nil
+  | y :: xs' => y :: snoc x xs'
+  end.
 
 (* Get an indexed element from a list, starting from 0.
    This is like the Coq 'nth' function, but returns an option instead
    of a provided default value. Using an option is useful when we simply
    want to determine whether some element is in the list, but don't
    need the actual value *)
-Fixpoint get {A: Type} (i: nat) (e: list A) {struct e}: option A :=
- match e, i with
- | x :: _,  O     => Some x
- | _ :: xs, S i'  => get  i' xs
- | _, _           => None
- end.
+Fixpoint get {A : Type} (i : nat) (e : list A) {struct e}: 
+option A :=
+  match e, i with
+  | x :: _, O => Some x
+  | _ :: xs, S i' => get i' xs
+  | _, _ => None
+  end.
 
 (** Remove all instances of a given string [s] from a list of strings [l]. *)
-Fixpoint rm (s:string) (l:list string) :=
-  match l with
-  | nil => nil
-  | y::tl => if (string_dec s y) then tl else y::(rm s tl)
-  end.
+Definition rm (s : string) (l : list string) := remove string_dec s l.
 
-Fixpoint is_in (s:string) (l:list string) : bool :=
+Fixpoint is_in (s : string) (l : list string): bool :=
   match l with
   | nil => false
-  | x::tl => if (string_dec x s) then true else is_in s tl
+  | x :: rest => if string_dec s x then true else is_in s rest
   end.
 
-Fixpoint append (l1:list string) (l2:list string) : list string :=
+(** Appends [l2] to [l1] removing duplicates from [l2]. *)
+Fixpoint append (l1 : list string) (l2 : list string): 
+list string :=
   match l2 with
   | nil => l1
-  | x::tl => append (if is_in x l1 then l1 else snoc x l1) tl
+  | x :: tl2 => append (if is_in x l1 then l1 else snoc x l1) tl2
   end.
 
 Open Scope string_scope.
 Example append_ex1 :
-  append (cons "a" (cons "b" nil))
-         (cons "x" (cons "y" nil))
-   = "a" :: "b" :: "x" :: "y" :: nil.
+  append (cons "a" (cons "b" nil)) (cons "x" (cons "y" nil)) =
+  "a" :: "b" :: "x" :: "y" :: nil.
+Proof. reflexivity. Qed.
+
+Example append_ex2 :
+  append (cons "a" (cons "b" nil)) (cons "x" (cons "b" nil)) =
+  "a" :: "b" :: "x" :: nil.
+Proof. reflexivity. Qed.
+
+Example append_ex3 :
+  append (cons "a" (cons "b" nil)) (cons "a" (cons "y" nil)) =
+  "a" :: "b" :: "y" :: nil.
 Proof. reflexivity. Qed.
 Close Scope string_scope.
+
+
+
+Require String. Open Scope string_scope.
+
+Ltac move_to_top x :=
+  match reverse goal with
+  | H:_ |- _ => try move x after H
+  end.
+
+Tactic Notation
+  "assert_eq" ident(x) constr(v) :=
+  let H := fresh in
+  assert (x = v) as H by reflexivity; clear H.
+
+Tactic Notation "Case_aux" ident(x) constr(name) :=
+  first [
+    set (x := name); move_to_top x
+  | assert_eq x name; move_to_top x
+  | fail 1 "because we are working on a different case" ].
+
+Tactic Notation "Case" constr(name) := Case_aux Case name.
+Tactic Notation "SCase" constr(name) := Case_aux SCase name.
+Tactic Notation "SSCase" constr(name) := Case_aux SSCase name.
+Tactic Notation "SSSCase" constr(name) := Case_aux SSSCase name.
+Tactic Notation "SSSSCase" constr(name) := Case_aux SSSSCase name.
+Tactic Notation "SSSSSCase" constr(name) := Case_aux SSSSSCase name.
+Tactic Notation "SSSSSSCase" constr(name) := Case_aux SSSSSSCase name.
+Tactic Notation "SSSSSSSCase" constr(name) := Case_aux SSSSSSSCase name.
+
+(**
+Binary relation utilities, specifically the [multi] closure of a relation.
+*)
+Definition relation (X : Type) := X -> X -> Prop.
+
+Definition deterministic {X : Type} (R : relation X) :=
+  forall x y1 y2 : X, R x y1 -> R x y2 -> y1 = y2. 
+
+Inductive multi (X : Type) (R : relation X) : X -> X -> Prop :=
+  | multi_refl : forall x : X, multi X R x x
+  | multi_step : forall x y z : X, R x y -> multi X R y z -> multi X R x z.
+Implicit Arguments  multi [[X]]. 
+
+Tactic Notation "multi_cases" tactic(first) ident(c) :=
+  first;
+  [ Case_aux c "multi_refl" | Case_aux c "multi_step" ].
+
+Theorem multi_R :
+ forall (X : Type) (R : relation X) (x y : X), R x y -> multi R x y.
+Proof.
+  intros X R x y r.
+  apply multi_step with y. apply r. apply multi_refl.   Qed.
+
+Theorem multi_trans :
+ forall (X : Type) (R : relation X) (x y z : X),
+ multi R x y -> multi R y z -> multi R x z.
+Proof.
+  intuition.
+  induction H.
+  - assumption.
+  - apply multi_step with y. assumption.
+    apply IHmulti. assumption. 
+Qed.
